WP rules - IsPtr Jnz and Restrict

theories/rules/rules_IsPtr.v
@@ -14,30 +14,30 @@ Section cap_lang_rules.
   Implicit Types r : RegName.
   Implicit Types v : cap_lang.val. 
   Implicit Types w : Word.
-  Implicit Types reg : gmap RegName Word.
+  Implicit Types reg : gmap (CoreN * RegName) Word.
   Implicit Types ms : gmap Addr Word.
 
-  Inductive IsPtr_spec (regs: Reg) (dst src: RegName) (regs': Reg): cap_lang.val -> Prop :=
+  Inductive IsPtr_spec (i: CoreN) (regs: Reg) (dst src: RegName) (regs': Reg): cap_lang.val -> Prop :=
   | IsPtr_spec_success (w: Word):
-      regs !! src = Some w →
-      incrementPC (<[ dst := WInt (if is_cap w then 1%Z else 0%Z) ]> regs) = Some regs' ->
-      IsPtr_spec regs dst src regs' NextIV
+      regs !! (i, src) = Some w →
+      incrementPC (<[ (i, dst) := WInt (if is_cap w then 1%Z else 0%Z) ]> regs) i = Some regs' ->
+      IsPtr_spec i regs dst src regs' (i, NextIV)
   | IsPtr_spec_failure (w: Word):
-      regs !! src = Some w →
-      incrementPC (<[ dst := WInt (if is_cap w then 1%Z else 0%Z) ]> regs) = None ->
-      IsPtr_spec regs dst src regs' FailedV.
+      regs !! (i, src) = Some w →
+      incrementPC (<[ (i, dst) := WInt (if is_cap w then 1%Z else 0%Z) ]> regs) i = None ->
+      IsPtr_spec i regs dst src regs' (i, FailedV).
 
-  Lemma wp_IsPtr Ep pc_p pc_b pc_e pc_a w dst src regs :
+  Lemma wp_IsPtr Ep i pc_p pc_b pc_e pc_a w dst src regs :
     decodeInstrW w = IsPtr dst src ->
     isCorrectPC (WCap pc_p pc_b pc_e pc_a) →
-    regs !! PC = Some (WCap pc_p pc_b pc_e pc_a) →
-    regs_of (IsPtr dst src) ⊆ dom _ regs →
+    regs !! (i, PC) = Some (WCap pc_p pc_b pc_e pc_a) →
+    regs_of_core (IsPtr dst src) i ⊆ dom _ regs →
     
     {{{ ▷ pc_a ↦ₐ w ∗
         ▷ [∗ map] k↦y ∈ regs, k ↦ᵣ y }}}
-      Instr Executable @ Ep
+      (i, Instr Executable) @ Ep
     {{{ regs' retv, RET retv;
-        ⌜ IsPtr_spec regs dst src regs' retv ⌝ ∗
+        ⌜ IsPtr_spec i regs dst src regs' retv ⌝ ∗
           pc_a ↦ₐ w ∗
           [∗ map] k↦y ∈ regs', k ↦ᵣ y }}}.
   Proof.
@@ -51,18 +51,21 @@ Section cap_lang_rules.
     iModIntro. iSplitR. by iPureIntro; apply normal_always_head_reducible.
     iNext. iIntros (e2 σ2 efs Hpstep).
     apply prim_step_exec_inv in Hpstep as (-> & -> & (c & -> & Hstep)).
-    iSplitR; auto. eapply step_exec_inv in Hstep; eauto.
+    iSplitR; auto. eapply core_step_exec_inv in Hstep; eauto.
     unfold exec in Hstep.
 
     specialize (indom_regs_incl _ _ _ Dregs Hregs) as Hri. unfold regs_of in Hri.
-    destruct (Hri dst) as [wdst [H'dst Hdst]]. by set_solver+.
-    destruct (Hri src) as [wsrc [H'src Hsrc]]. by set_solver+.
+    destruct (Hri i dst) as [wdst [H'dst Hdst]]. by set_solver+.
+    destruct (Hri i src) as [wsrc [H'src Hsrc]]. by set_solver+.
 
-    assert (exec_opt (IsPtr dst src) (r, m) = updatePC (update_reg (r, m) dst (WInt (if is_cap wsrc then 1%Z else 0%Z)))) as HH.
+    assert (exec_opt (IsPtr dst src) i (r, m)
+            = updatePC i
+                (update_reg (r, m) i dst
+                   (WInt (if is_cap wsrc then 1%Z else 0%Z)))) as HH.
     {  rewrite /= Hsrc. unfold is_cap; destruct wsrc; auto. }
     rewrite HH in Hstep. rewrite /update_reg /= in Hstep.
 
-    destruct (incrementPC (<[ dst := WInt (if is_cap wsrc then 1%Z else 0%Z) ]> regs))
+    destruct (incrementPC (<[ (i, dst) := WInt (if is_cap wsrc then 1%Z else 0%Z) ]> regs) i)
       as [regs'|] eqn:Hregs'; pose proof Hregs' as H'regs'; cycle 1.
     { apply incrementPC_fail_updatePC with (m:=m) in Hregs'.
       eapply updatePC_fail_incl with (m':=m) in Hregs'.
@@ -74,103 +77,109 @@ Section cap_lang_rules.
 
     (* Success *)
 
-    eapply (incrementPC_success_updatePC _ m) in Hregs'
+    eapply (incrementPC_success_updatePC _ i m) in Hregs'
       as (p' & g' & b' & e' & a'' & a_pc' & HPC'' & HuPC & ->).
     eapply updatePC_success_incl with (m':=m) in HuPC. 2: by eapply insert_mono; eauto. rewrite HuPC in Hstep.
 
     simplify_pair_eq. iFrame.
-    iMod ((gen_heap_update_inSepM _ _ dst) with "Hr Hmap") as "[Hr Hmap]"; eauto.
-    iMod ((gen_heap_update_inSepM _ _ PC) with "Hr Hmap") as "[Hr Hmap]"; eauto.
+    iMod ((gen_heap_update_inSepM _ _ (i, dst)) with "Hr Hmap") as "[Hr Hmap]"; eauto.
+    iMod ((gen_heap_update_inSepM _ _ (i, PC)) with "Hr Hmap") as "[Hr Hmap]"; eauto.
     iFrame. iModIntro. iApply "Hφ". iFrame. iPureIntro. econstructor; eauto.
   Qed.
 
-  Lemma wp_IsPtr_successPC E pc_p pc_b pc_e pc_a pc_a' w dst w' :
+  Lemma wp_IsPtr_successPC E i pc_p pc_b pc_e pc_a pc_a' w dst w' :
     decodeInstrW w = IsPtr dst PC →
     isCorrectPC (WCap pc_p pc_b pc_e pc_a) →
     (pc_a + 1)%a = Some pc_a' →
 
-    {{{ ▷ PC ↦ᵣ WCap pc_p pc_b pc_e pc_a
+    {{{ ▷ (i, PC) ↦ᵣ WCap pc_p pc_b pc_e pc_a
         ∗ ▷ pc_a ↦ₐ w
-        ∗ ▷ dst ↦ᵣ w'
+        ∗ ▷ (i, dst) ↦ᵣ w'
     }}}
-      Instr Executable @ E
-      {{{ RET NextIV;
-          PC ↦ᵣ WCap pc_p pc_b pc_e pc_a'
+      (i, Instr Executable) @ E
+      {{{ RET (i, NextIV);
+          (i, PC) ↦ᵣ WCap pc_p pc_b pc_e pc_a'
           ∗ pc_a ↦ₐ w
-          ∗ dst ↦ᵣ WInt 1%Z }}}.
+          ∗ (i, dst) ↦ᵣ WInt 1%Z }}}.
    Proof.
      iIntros (Hinstr Hvpc Hpca' ϕ) "(>HPC & >Hpc_a & >Hdst) Hφ".
      iDestruct (map_of_regs_2 with "HPC Hdst") as "[Hmap %]".
-     iApply (wp_IsPtr with "[$Hmap Hpc_a]"); eauto; simplify_map_eq; eauto.
+     iApply (wp_IsPtr with "[$Hmap Hpc_a]"); eauto; simplify_map_eq by simplify_pair_eq; eauto.
      by rewrite !dom_insert; set_solver+.
      iNext. iIntros (regs' retv) "(#Hspec & Hpc_a & Hmap)". iDestruct "Hspec" as %Hspec.
 
      destruct Hspec as [|].
-     { iApply "Hφ". iFrame. incrementPC_inv; simplify_map_eq.
-       rewrite (insert_commute _ PC dst) // insert_insert insert_commute // insert_insert.
+     { iApply "Hφ". iFrame. incrementPC_inv; simplify_map_eq by simplify_pair_eq.
+       rewrite (insert_commute _ (i, PC) (i, dst)) ; simplify_pair_eq.
+       rewrite insert_insert (insert_commute _ (i, PC) (i, dst)) ; simplify_pair_eq.
+       rewrite insert_insert.
        iDestruct (regs_of_map_2 with "Hmap") as "(?&?)"; eauto; iFrame. }
-     { incrementPC_inv; simplify_map_eq; eauto. congruence. }
+     { incrementPC_inv; simplify_map_eq by simplify_pair_eq; eauto. congruence. }
    Qed.
 
-   Lemma wp_IsPtr_success E pc_p pc_b pc_e pc_a pc_a' w dst r wr w' :
+   Lemma wp_IsPtr_success E i pc_p pc_b pc_e pc_a pc_a' w dst r wr w' :
      decodeInstrW w = IsPtr dst r →
      isCorrectPC (WCap pc_p pc_b pc_e pc_a) →
      (pc_a + 1)%a = Some pc_a' →
 
-       {{{ ▷ PC ↦ᵣ WCap pc_p pc_b pc_e pc_a
+       {{{ ▷ (i, PC) ↦ᵣ WCap pc_p pc_b pc_e pc_a
              ∗ ▷ pc_a ↦ₐ w
-             ∗ ▷ r ↦ᵣ wr
-             ∗ ▷ dst ↦ᵣ w'
+             ∗ ▷(i, r)↦ᵣ wr
+             ∗ ▷ (i, dst) ↦ᵣ w'
        }}}
-         Instr Executable @ E
-       {{{ RET NextIV;
-           PC ↦ᵣ WCap pc_p pc_b pc_e pc_a'
+         (i, Instr Executable) @ E
+       {{{ RET (i, NextIV);
+           (i, PC) ↦ᵣ WCap pc_p pc_b pc_e pc_a'
            ∗ pc_a ↦ₐ w
-           ∗ r ↦ᵣ wr
-           ∗ dst ↦ᵣ WInt (if is_cap wr then 1%Z else 0%Z) }}}.
+           ∗(i, r)↦ᵣ wr
+           ∗ (i, dst) ↦ᵣ WInt (if is_cap wr then 1%Z else 0%Z) }}}.
    Proof.
     iIntros (Hinstr Hvpc Hpc_a ϕ) "(>HPC & >Hpc_a & >Hr & >Hdst) Hφ".
     iDestruct (map_of_regs_3 with "HPC Hr Hdst") as "[Hmap (%&%&%)]".
-    iApply (wp_IsPtr with "[$Hmap Hpc_a]"); eauto; simplify_map_eq; eauto.
+    iApply (wp_IsPtr with "[$Hmap Hpc_a]"); eauto; simplify_map_eq by simplify_pair_eq; eauto.
     by rewrite !dom_insert; set_solver+.
     iNext. iIntros (regs' retv) "(#Hspec & Hpc_a & Hmap)". iDestruct "Hspec" as %Hspec.
 
     destruct Hspec as [|].
     { (* Success *)
-      iApply "Hφ". iFrame. incrementPC_inv; simplify_map_eq.
-      rewrite (insert_commute _ PC dst) // insert_insert (insert_commute _ r dst) //
-              (insert_commute _ dst PC) // insert_insert.
-      iDestruct (regs_of_map_3 with "Hmap") as "(?&?&?)"; eauto; iFrame. }
+      iApply "Hφ". iFrame. incrementPC_inv; simplify_map_eq by simplify_pair_eq.
+       rewrite (insert_commute _ (i, PC) (i, dst)) ; simplify_pair_eq.
+       rewrite insert_insert (insert_commute _ (i, r) (i, dst)) ; simplify_pair_eq.
+       rewrite (insert_commute _ (i, dst) (i, PC)) ; simplify_pair_eq.
+       rewrite insert_insert.
+       iDestruct (regs_of_map_3 with "Hmap") as "(?&?&?)"; eauto; iFrame. }
     { (* Failure (contradiction) *)
-      incrementPC_inv; simplify_map_eq; eauto. congruence. }
+      incrementPC_inv; simplify_map_eq by simplify_pair_eq; eauto. congruence. }
    Qed.
 
-   Lemma wp_IsPtr_success_dst E pc_p pc_b pc_e pc_a pc_a' w dst w' :
+   Lemma wp_IsPtr_success_dst E i pc_p pc_b pc_e pc_a pc_a' w dst w' :
      decodeInstrW w = IsPtr dst dst →
      isCorrectPC (WCap pc_p pc_b pc_e pc_a) →
      (pc_a + 1)%a = Some pc_a' →
      
-       {{{ ▷ PC ↦ᵣ WCap pc_p pc_b pc_e pc_a
+       {{{ ▷ (i, PC) ↦ᵣ WCap pc_p pc_b pc_e pc_a
              ∗ ▷ pc_a ↦ₐ w
-             ∗ ▷ dst ↦ᵣ w'
+             ∗ ▷ (i, dst) ↦ᵣ w'
        }}}
-         Instr Executable @ E
-       {{{ RET NextIV;
-           PC ↦ᵣ WCap pc_p pc_b pc_e pc_a'
+         (i, Instr Executable) @ E
+       {{{ RET (i, NextIV);
+           (i, PC) ↦ᵣ WCap pc_p pc_b pc_e pc_a'
            ∗ pc_a ↦ₐ w
-           ∗ dst ↦ᵣ WInt (if is_cap w' then 1%Z else 0%Z) }}}.
+           ∗ (i, dst) ↦ᵣ WInt (if is_cap w' then 1%Z else 0%Z) }}}.
    Proof.
      iIntros (Hinstr Hvpc Hpca' ϕ) "(>HPC & >Hpc_a & >Hdst) Hφ".
      iDestruct (map_of_regs_2 with "HPC Hdst") as "[Hmap %]".
-     iApply (wp_IsPtr with "[$Hmap Hpc_a]"); eauto; simplify_map_eq; eauto.
+     iApply (wp_IsPtr with "[$Hmap Hpc_a]"); eauto; simplify_map_eq by simplify_pair_eq; eauto.
      by rewrite !dom_insert; set_solver+.
      iNext. iIntros (regs' retv) "(#Hspec & Hpc_a & Hmap)". iDestruct "Hspec" as %Hspec.
 
      destruct Hspec as [|].
-     { iApply "Hφ". iFrame. incrementPC_inv; simplify_map_eq.
-       rewrite (insert_commute _ PC dst) // insert_insert insert_commute // insert_insert.
+     { iApply "Hφ". iFrame. incrementPC_inv; simplify_map_eq by simplify_pair_eq.
+       rewrite (insert_commute _ (i, PC) (i, dst)) ; simplify_pair_eq.
+       rewrite insert_insert (insert_commute _ (i, PC) (i, dst)) ; simplify_pair_eq.
+       rewrite insert_insert.
        iDestruct (regs_of_map_2 with "Hmap") as "(?&?)"; eauto; iFrame. }
-     { incrementPC_inv; simplify_map_eq; eauto. congruence. }
+     { incrementPC_inv; simplify_map_eq by simplify_pair_eq; eauto. congruence. }
    Qed.
 
 End cap_lang_rules.
