theories/rules/rules_Jnz.v
@@ -14,37 +14,37 @@ Section cap_lang_rules.
   Implicit Types r : RegName.
   Implicit Types v : cap_lang.val. 
   Implicit Types w : Word.
-  Implicit Types reg : gmap RegName Word.
+  Implicit Types reg : gmap (CoreN * RegName) Word.
   Implicit Types ms : gmap Addr Word.
 
-  Inductive Jnz_spec (regs: Reg) (dst src: RegName) : Reg → cap_lang.val → Prop :=
+  Inductive Jnz_spec (i: CoreN) (regs: Reg) (dst src: RegName) : Reg → cap_lang.val → Prop :=
   | Jnz_spec_failure w:
-      regs !! src = Some w →
+      regs !! (i, src) = Some w →
       nonZero w = false →
-      incrementPC regs = None →
-      Jnz_spec regs dst src regs FailedV
+      incrementPC regs i = None →
+      Jnz_spec i regs dst src regs (i, FailedV)
   | Jnz_spec_success1 w regs':
-      regs !! src = Some w →
+      regs !! (i, src) = Some w →
       nonZero w = false →
-      incrementPC regs = Some regs' →
-      Jnz_spec regs dst src regs' NextIV
+      incrementPC regs i = Some regs' →
+      Jnz_spec i regs dst src regs' (i, NextIV)
   | Jnz_spec_success2 w w':
-      regs !! src = Some w →
-      regs !! dst = Some w' →
+      regs !! (i, src) = Some w →
+      regs !! (i, dst) = Some w' →
       nonZero w = true →
-      Jnz_spec regs dst src (<[PC := updatePcPerm w' ]> regs) NextIV.
+      Jnz_spec i regs dst src (<[(i, PC) := updatePcPerm w' ]> regs) (i, NextIV).
 
-  Lemma wp_Jnz Ep pc_p pc_b pc_e pc_a w dst src regs :
+  Lemma wp_Jnz Ep i pc_p pc_b pc_e pc_a w dst src regs :
     decodeInstrW w = Jnz dst src ->
     isCorrectPC (WCap pc_p pc_b pc_e pc_a) →
-    regs !! PC = Some (WCap pc_p pc_b pc_e pc_a) →
-    regs_of (Jnz dst src) ⊆ dom _ regs →
+    regs !! (i, PC) = Some (WCap pc_p pc_b pc_e pc_a) →
+    regs_of_core (Jnz dst src) i ⊆ dom _ regs →
     
     {{{ ▷ pc_a ↦ₐ w ∗
         ▷ [∗ map] k↦y ∈ regs, k ↦ᵣ y }}}
-      Instr Executable @ Ep
+      (i, Instr Executable) @ Ep
     {{{ regs' retv, RET retv;
-        ⌜ Jnz_spec regs dst src regs' retv ⌝ ∗
+        ⌜ Jnz_spec i regs dst src regs' retv ⌝ ∗
         pc_a ↦ₐ w ∗
         [∗ map] k↦y ∈ regs', k ↦ᵣ y }}}.
   Proof.
@@ -58,54 +58,54 @@ Section cap_lang_rules.
     iModIntro. iSplitR. by iPureIntro; apply normal_always_head_reducible.
     iNext. iIntros (e2 σ2 efs Hpstep).
     apply prim_step_exec_inv in Hpstep as (-> & -> & (c & -> & Hstep)).
-    iSplitR; auto. eapply step_exec_inv in Hstep; eauto.
+    iSplitR; auto. eapply core_step_exec_inv in Hstep; eauto.
 
     specialize (indom_regs_incl _ _ _ Dregs Hregs) as Hri.
     unfold regs_of in Hri, Dregs.
-    destruct (Hri src) as [wsrc [H'src Hsrc]]. by set_solver+.
-    destruct (Hri dst) as [wdst [H'dst Hdst]]. by set_solver+.
+    destruct (Hri i src) as [wsrc [H'src Hsrc]]. by set_solver+.
+    destruct (Hri i dst) as [wdst [H'dst Hdst]]. by set_solver+.
     unfold exec in Hstep; cbn in Hstep.
 
     destruct (nonZero wsrc) eqn:Hnz; pose proof Hnz as H'nz;
       cbn in Hstep; rewrite Hsrc Hdst /= Hnz in Hstep.
     { inv Hstep. simplify_pair_eq.
-      iMod ((gen_heap_update_inSepM _ _ PC) with "Hr Hmap") as "[Hr Hmap]"; eauto.
+      iMod ((gen_heap_update_inSepM _ _ (i, PC)) with "Hr Hmap") as "[Hr Hmap]"; eauto.
       iFrame. iApply "Hφ". iFrame. iPureIntro. econstructor 3; eauto. }
 
-    destruct (incrementPC regs) eqn:HX; pose proof HX as H'X; cycle 1.
+    destruct (incrementPC regs i) eqn:HX; pose proof HX as H'X; cycle 1.
     { apply incrementPC_fail_updatePC with (m:=m) in HX.
       eapply updatePC_fail_incl with (m':=m) in HX; eauto.
       rewrite HX in Hstep. inv Hstep.
       iFrame. iApply "Hφ". iFrame. iPureIntro; econstructor; eauto. }
 
-    destruct (incrementPC_success_updatePC _ m _ HX)
+    destruct (incrementPC_success_updatePC _ i m _ HX)
       as (p' & g' & b' & e' & a'' & a_pc' & HPC'' & HuPC & ->).
     eapply updatePC_success_incl with (m':=m) in HuPC; eauto. rewrite HuPC in Hstep.
     simplify_pair_eq.
-    iMod ((gen_heap_update_inSepM _ _ PC) with "Hr Hmap") as "[Hr Hmap]"; eauto.
+    iMod ((gen_heap_update_inSepM _ _ (i, PC)) with "Hr Hmap") as "[Hr Hmap]"; eauto.
     iFrame. iApply "Hφ". iFrame. iPureIntro. econstructor 2; eauto.
   Qed.
 
-  Lemma wp_jnz_success_jmp E r1 r2 pc_p pc_b pc_e pc_a w w1 w2 :
+  Lemma wp_jnz_success_jmp E i r1 r2 pc_p pc_b pc_e pc_a w w1 w2 :
     decodeInstrW w = Jnz r1 r2 →
     isCorrectPC (WCap pc_p pc_b pc_e pc_a) →
     w2 ≠ WInt 0%Z →
 
-    {{{ ▷ PC ↦ᵣ WCap pc_p pc_b pc_e pc_a
+    {{{ ▷ (i, PC) ↦ᵣ WCap pc_p pc_b pc_e pc_a
         ∗ ▷ pc_a ↦ₐ w
-        ∗ ▷ r1 ↦ᵣ w1
-        ∗ ▷ r2 ↦ᵣ w2 }}}
-      Instr Executable @ E
-      {{{ RET NextIV;
-          PC ↦ᵣ updatePcPerm w1
+        ∗ ▷ (i, r1) ↦ᵣ w1
+        ∗ ▷ (i, r2) ↦ᵣ w2 }}}
+      (i, Instr Executable) @ E
+      {{{ RET (i, NextIV);
+          (i, PC) ↦ᵣ updatePcPerm w1
           ∗ pc_a ↦ₐ w
-          ∗ r1 ↦ᵣ w1
-          ∗ r2 ↦ᵣ w2 }}}.
+          ∗ (i, r1) ↦ᵣ w1
+          ∗ (i, r2) ↦ᵣ w2 }}}.
   Proof.
     iIntros (Hinstr Hvpc Hne ϕ) "(>HPC & >Hpc_a & >Hr1 & >Hr2) Hφ".
     iDestruct (map_of_regs_3 with "HPC Hr1 Hr2") as "[Hmap (%&%&%)]".
     iApply (wp_Jnz with "[$Hmap Hpc_a]"); eauto; simplify_map_eq; eauto.
-    by unfold regs_of; rewrite !dom_insert; set_solver+.
+    by unfold regs_of_core; rewrite !dom_insert; set_solver+.
     iNext. iIntros (regs' retv) "(#Hspec & Hpc_a & Hmap)". iDestruct "Hspec" as %Hspec.
 
     assert (nonZero w2 = true).
@@ -114,30 +114,30 @@ Section cap_lang_rules.
       apply Hne. f_equal. by apply Z.compare_eq. }
 
    destruct Hspec as [ | | ].
-   { exfalso. simplify_map_eq. congruence. }
-   { exfalso. simplify_map_eq. congruence. }
-   { iApply "Hφ". iFrame. simplify_map_eq. rewrite insert_insert.
+   { exfalso. simplify_map_eq by simplify_pair_eq. congruence. }
+   { exfalso. simplify_map_eq by simplify_pair_eq. congruence. }
+   { iApply "Hφ". iFrame. simplify_map_eq by simplify_pair_eq. rewrite insert_insert.
      iDestruct (regs_of_map_3 with "Hmap") as "(?&?&?)"; eauto; iFrame. }
   Qed.
 
-  Lemma wp_jnz_success_jmp2 E r2 pc_p pc_b pc_e pc_a w w2 :
+  Lemma wp_jnz_success_jmp2 E i r2 pc_p pc_b pc_e pc_a w w2 :
     decodeInstrW w = Jnz r2 r2 →
     isCorrectPC (WCap pc_p pc_b pc_e pc_a) →
     w2 ≠ WInt 0%Z →
 
-    {{{ ▷ PC ↦ᵣ WCap pc_p pc_b pc_e pc_a
+    {{{ ▷ (i, PC) ↦ᵣ WCap pc_p pc_b pc_e pc_a
         ∗ ▷ pc_a ↦ₐ w
-        ∗ ▷ r2 ↦ᵣ w2 }}}
-      Instr Executable @ E
-      {{{ RET NextIV;
-          PC ↦ᵣ updatePcPerm w2
+        ∗ ▷ (i, r2) ↦ᵣ w2 }}}
+      (i, Instr Executable) @ E
+      {{{ RET (i, NextIV);
+          (i, PC) ↦ᵣ updatePcPerm w2
           ∗ pc_a ↦ₐ w
-          ∗ r2 ↦ᵣ w2 }}}.
+          ∗ (i, r2) ↦ᵣ w2 }}}.
   Proof.
     iIntros (Hinstr Hvpc Hne ϕ) "(>HPC & >Hpc_a & >Hr2) Hφ".
     iDestruct (map_of_regs_2 with "HPC Hr2") as "[Hmap %]".
-    iApply (wp_Jnz with "[$Hmap Hpc_a]"); eauto; simplify_map_eq; eauto.
-    by unfold regs_of; rewrite !dom_insert; set_solver+.
+    iApply (wp_Jnz with "[$Hmap Hpc_a]"); eauto; simplify_map_eq by simplify_pair_eq; eauto.
+    by unfold regs_of_core; rewrite !dom_insert; set_solver+.
     iNext. iIntros (regs' retv) "(#Hspec & Hpc_a & Hmap)". iDestruct "Hspec" as %Hspec.
 
     assert (nonZero w2 = true).
@@ -146,52 +146,52 @@ Section cap_lang_rules.
       apply Hne. f_equal. by apply Z.compare_eq. }
 
    destruct Hspec as [ | | ].
-   { exfalso. simplify_map_eq. congruence. }
-   { exfalso. simplify_map_eq. congruence. }
-   { iApply "Hφ". iFrame. simplify_map_eq. rewrite insert_insert.
+   { exfalso. simplify_map_eq by simplify_pair_eq. congruence. }
+   { exfalso. simplify_map_eq by simplify_pair_eq. congruence. }
+   { iApply "Hφ". iFrame. simplify_map_eq by simplify_pair_eq. rewrite insert_insert.
      iDestruct (regs_of_map_2 with "Hmap") as "(?&?)"; eauto; iFrame. }
   Qed.
 
-  Lemma wp_jnz_success_jmpPC E pc_p pc_b pc_e pc_a w :
+  Lemma wp_jnz_success_jmpPC E i pc_p pc_b pc_e pc_a w :
     decodeInstrW w = Jnz PC PC →
     isCorrectPC (WCap pc_p pc_b pc_e pc_a) →
 
-    {{{ ▷ PC ↦ᵣ WCap pc_p pc_b pc_e pc_a
+    {{{ ▷ (i, PC) ↦ᵣ WCap pc_p pc_b pc_e pc_a
         ∗ ▷ pc_a ↦ₐ w }}}
-      Instr Executable @ E
-      {{{ RET NextIV;
-          PC ↦ᵣ updatePcPerm (WCap pc_p pc_b pc_e pc_a)
+      (i, Instr Executable) @ E
+      {{{ RET (i, NextIV);
+          (i, PC) ↦ᵣ updatePcPerm (WCap pc_p pc_b pc_e pc_a)
           ∗ pc_a ↦ₐ w }}}.
   Proof.
     iIntros (Hinstr Hvpc ϕ) "(>HPC & >Hpc_a) Hφ".
     iDestruct (map_of_regs_1 with "HPC") as "Hmap".
-    iApply (wp_Jnz with "[$Hmap Hpc_a]"); eauto; simplify_map_eq; eauto.
-    by unfold regs_of; rewrite !dom_insert; set_solver+.
+    iApply (wp_Jnz with "[$Hmap Hpc_a]"); eauto; simplify_map_eq by simplify_pair_eq; eauto.
+    by unfold regs_of_core; rewrite !dom_insert; set_solver+.
     iNext. iIntros (regs' retv) "(#Hspec & Hpc_a & Hmap)". iDestruct "Hspec" as %Hspec.
 
-   destruct Hspec as [ | | ]; [ by simplify_map_eq .. | ].
-   { iApply "Hφ". iFrame. simplify_map_eq. rewrite insert_insert.
+   destruct Hspec as [ | | ]; [ by simplify_map_eq by simplify_pair_eq .. | ].
+   { iApply "Hφ". iFrame. simplify_map_eq by simplify_pair_eq. rewrite insert_insert.
      iDestruct (regs_of_map_1 with "Hmap") as "?"; eauto; iFrame. }
   Qed.
 
-  Lemma wp_jnz_success_jmpPC1 E r2 pc_p pc_b pc_e pc_a w w2 :
+  Lemma wp_jnz_success_jmpPC1 E i r2 pc_p pc_b pc_e pc_a w w2 :
     decodeInstrW w = Jnz PC r2 →
     isCorrectPC (WCap pc_p pc_b pc_e pc_a) →
     w2 ≠ WInt 0%Z →
 
-    {{{ ▷ PC ↦ᵣ WCap pc_p pc_b pc_e pc_a
+    {{{ ▷ (i, PC) ↦ᵣ WCap pc_p pc_b pc_e pc_a
         ∗ ▷ pc_a ↦ₐ w
-        ∗ ▷ r2 ↦ᵣ w2 }}}
-      Instr Executable @ E
-      {{{ RET NextIV;
-          PC ↦ᵣ updatePcPerm (WCap pc_p pc_b pc_e pc_a)
+        ∗ ▷ (i, r2) ↦ᵣ w2 }}}
+      (i, Instr Executable) @ E
+      {{{ RET (i, NextIV);
+          (i, PC) ↦ᵣ updatePcPerm (WCap pc_p pc_b pc_e pc_a)
           ∗ pc_a ↦ₐ w
-          ∗ r2 ↦ᵣ w2 }}}.
+          ∗ (i, r2) ↦ᵣ w2 }}}.
   Proof.
     iIntros (Hinstr Hvpc Hne ϕ) "(>HPC & >Hpc_a & >Hr2) Hφ".
     iDestruct (map_of_regs_2 with "HPC Hr2") as "[Hmap %]".
-    iApply (wp_Jnz with "[$Hmap Hpc_a]"); eauto; simplify_map_eq; eauto.
-    by unfold regs_of; rewrite !dom_insert; set_solver+.
+    iApply (wp_Jnz with "[$Hmap Hpc_a]"); eauto; simplify_map_eq by simplify_pair_eq; eauto.
+    by unfold regs_of_core; rewrite !dom_insert; set_solver+.
     iNext. iIntros (regs' retv) "(#Hspec & Hpc_a & Hmap)". iDestruct "Hspec" as %Hspec.
 
     assert (nonZero w2 = true).
@@ -200,59 +200,59 @@ Section cap_lang_rules.
       apply Hne. f_equal. by apply Z.compare_eq. }
 
    destruct Hspec as [ | | ].
-   { exfalso. simplify_map_eq. congruence. }
-   { exfalso. simplify_map_eq. congruence. }
-   { iApply "Hφ". iFrame. simplify_map_eq. rewrite insert_insert.
+   { exfalso. simplify_map_eq by simplify_pair_eq. congruence. }
+   { exfalso. simplify_map_eq by simplify_pair_eq. congruence. }
+   { iApply "Hφ". iFrame. simplify_map_eq by simplify_pair_eq. rewrite insert_insert.
      iDestruct (regs_of_map_2 with "Hmap") as "(?&?)"; eauto; iFrame. }
   Qed.
 
-  Lemma wp_jnz_success_jmpPC2 E r1 pc_p pc_b pc_e pc_a w w1 :
+  Lemma wp_jnz_success_jmpPC2 E i r1 pc_p pc_b pc_e pc_a w w1 :
     decodeInstrW w = Jnz r1 PC →
     isCorrectPC (WCap pc_p pc_b pc_e pc_a) →
 
-    {{{ ▷ PC ↦ᵣ WCap pc_p pc_b pc_e pc_a
+    {{{ ▷ (i, PC) ↦ᵣ WCap pc_p pc_b pc_e pc_a
         ∗ ▷ pc_a ↦ₐ w
-        ∗ ▷ r1 ↦ᵣ w1 }}}
-      Instr Executable @ E
-      {{{ RET NextIV;
-          PC ↦ᵣ updatePcPerm w1
+        ∗ ▷ (i, r1) ↦ᵣ w1 }}}
+      (i, Instr Executable) @ E
+      {{{ RET (i, NextIV);
+          (i, PC) ↦ᵣ updatePcPerm w1
           ∗ pc_a ↦ₐ w
-          ∗ r1 ↦ᵣ w1 }}}.
+          ∗ (i, r1) ↦ᵣ w1 }}}.
   Proof.
     iIntros (Hinstr Hvpc ϕ) "(>HPC & >Hpc_a & >Hr1) Hφ".
     iDestruct (map_of_regs_2 with "HPC Hr1") as "[Hmap %]".
-    iApply (wp_Jnz with "[$Hmap Hpc_a]"); eauto; simplify_map_eq; eauto.
-    by unfold regs_of; rewrite !dom_insert; set_solver+.
+    iApply (wp_Jnz with "[$Hmap Hpc_a]"); eauto; simplify_map_eq by simplify_pair_eq; eauto.
+    by unfold regs_of_core; rewrite !dom_insert; set_solver+.
     iNext. iIntros (regs' retv) "(#Hspec & Hpc_a & Hmap)". iDestruct "Hspec" as %Hspec.
 
-   destruct Hspec as [ | | ]; [ by simplify_map_eq .. | ].
-   { iApply "Hφ". iFrame. simplify_map_eq. rewrite insert_insert.
+   destruct Hspec as [ | | ]; [ by simplify_map_eq by simplify_pair_eq .. | ].
+   { iApply "Hφ". iFrame. simplify_map_eq by simplify_pair_eq. rewrite insert_insert.
      iDestruct (regs_of_map_2 with "Hmap") as "(?&?)"; eauto; iFrame. }
   Qed.
 
-  Lemma wp_jnz_success_next E r1 r2 pc_p pc_b pc_e pc_a pc_a' w w1 :
+  Lemma wp_jnz_success_next E i r1 r2 pc_p pc_b pc_e pc_a pc_a' w w1 :
     decodeInstrW w = Jnz r1 r2 →
     isCorrectPC (WCap pc_p pc_b pc_e pc_a) →
     (pc_a + 1)%a = Some pc_a' →
 
-    {{{ ▷ PC ↦ᵣ WCap pc_p pc_b pc_e pc_a
+    {{{ ▷ (i, PC) ↦ᵣ WCap pc_p pc_b pc_e pc_a
         ∗ ▷ pc_a ↦ₐ w
-        ∗ ▷ r1 ↦ᵣ w1
-        ∗ ▷ r2 ↦ᵣ WInt 0%Z }}}
-      Instr Executable @ E
-      {{{ RET NextIV;
-          PC ↦ᵣ WCap pc_p pc_b pc_e pc_a'
+        ∗ ▷ (i, r1) ↦ᵣ w1
+        ∗ ▷ (i, r2) ↦ᵣ WInt 0%Z }}}
+      (i, Instr Executable) @ E
+      {{{ RET (i, NextIV);
+          (i, PC) ↦ᵣ WCap pc_p pc_b pc_e pc_a'
           ∗ pc_a ↦ₐ w
-          ∗ r1 ↦ᵣ w1
-          ∗ r2 ↦ᵣ WInt 0%Z }}}.
+          ∗ (i, r1) ↦ᵣ w1
+          ∗ (i, r2) ↦ᵣ WInt 0%Z }}}.
   Proof.
     iIntros (Hinstr Hvpc Hpc_a' ϕ) "(>HPC & >Hpc_a & >Hr1 & >Hr2) Hφ".
     iDestruct (map_of_regs_3 with "HPC Hr1 Hr2") as "[Hmap (%&%&%)]".
-    iApply (wp_Jnz with "[$Hmap Hpc_a]"); eauto; simplify_map_eq; eauto.
-    by unfold regs_of; rewrite !dom_insert; set_solver+.
+    iApply (wp_Jnz with "[$Hmap Hpc_a]"); eauto; simplify_map_eq by simplify_pair_eq; eauto.
+    by unfold regs_of_core; rewrite !dom_insert; set_solver+.
     iNext. iIntros (regs' retv) "(#Hspec & Hpc_a & Hmap)". iDestruct "Hspec" as %Hspec.
 
-   destruct Hspec as [ | | ]; try incrementPC_inv; simplify_map_eq; eauto.
+   destruct Hspec as [ | | ]; try incrementPC_inv; simplify_map_eq by simplify_pair_eq; eauto.
    { congruence. }
    { iApply "Hφ". iFrame. rewrite insert_insert.
      iDestruct (regs_of_map_3 with "Hmap") as "(?&?&?)"; eauto; iFrame. }
