theories/rules.v
@@ -1,11 +1,7 @@
-(* From cap_machine.rules Require Export *)
-(*      rules_Get rules_Load rules_Store rules_AddSubLt *)
-(*      rules_Lea rules_Mov rules_Restrict rules_IsPtr *)
-(*      rules_Jmp rules_Jnz rules_Subseg. *)
 From cap_machine.rules Require Export
      rules_Get rules_Load rules_Store rules_AddSubLt
-     rules_Lea rules_Mov
-     rules_Jmp rules_Subseg.
+     rules_Lea rules_Mov rules_Restrict rules_IsPtr
+     rules_Jmp rules_Jnz rules_Subseg.
 From iris.base_logic Require Export invariants gen_heap.
 From iris.program_logic Require Export weakestpre ectx_lifting.
 From cap_machine.rules Require Export rules_base.
